providers/quic/Impl.QUIC.fsti
@@ -1,0 +1,180 @@
+/// An implementation of Spec.QUIC.fst that is concerned only with functional
+/// correctness (no notion of model for now).
+module Impl.QUIC
+
+module G = FStar.Ghost
+module B = LowStar.Buffer
+module S = FStar.Seq
+module HS = FStar.HyperStack
+
+module U64 = FStar.UInt64
+module U32 = FStar.UInt32
+module U8 = FStar.UInt8
+
+open FStar.HyperStack
+open FStar.HyperStack.ST
+
+open EverCrypt.Helpers
+open EverCrypt.Error
+
+#set-options "--max_fuel 0 --max_ifuel 0"
+
+type role = | Reader | Writer
+
+unfold noextract
+let hash_alg = Spec.Hash.Definitions.hash_alg
+
+unfold noextract
+let aead_alg = Spec.AEAD.alg
+
+unfold noextract
+let lbytes = Spec.QUIC.lbytes
+
+/// This is not a cryptographic index; rather, this is just a regular type
+/// index, where instead of indexing on a single algorithm (like, say, AEAD), we
+/// index on three values.
+///
+/// The record is here to limit the profileration of hide/reveal in the stateful
+/// functions, and to give easier projectors (ADL, JP).
+type index = {
+  role: role;
+  hash_alg: Spec.Hash.Definitions.hash_alg;
+  aead_alg: Spec.AEAD.alg;
+}
+
+/// Boilerplate
+/// -----------
+
+[@CAbstractStruct]
+val state_s: index -> Type0
+
+let state i = B.pointer (state_s i)
+
+val footprint_s: #i:index -> state_s i -> GTot B.loc
+let footprint (#i:index) (m: HS.mem) (s: state i) =
+  B.(loc_union (loc_addr_of_buffer s) (footprint_s (B.deref m s)))
+
+let loc_includes_union_l_footprint_s
+  (l1 l2: B.loc) (#i: index) (s: state_s i)
+: Lemma
+  (requires (
+    B.loc_includes l1 (footprint_s s) \/ B.loc_includes l2 (footprint_s s)
+  ))
+  (ensures (B.loc_includes (B.loc_union l1 l2) (footprint_s s)))
+  [SMTPat (B.loc_includes (B.loc_union l1 l2) (footprint_s s))]
+= B.loc_includes_union_l l1 l2 (footprint_s s)
+
+val invariant_s: (#i:index) -> HS.mem -> state_s i -> Type0
+let invariant (#i:index) (m: HS.mem) (s: state i) =
+  B.live m s /\
+  B.(loc_disjoint (loc_addr_of_buffer s) (footprint_s (B.deref m s))) /\
+  invariant_s m (B.get m s 0)
+
+val invariant_loc_in_footprint
+  (#i: index)
+  (s: state i)
+  (m: HS.mem)
+: Lemma
+  (requires (invariant m s))
+  (ensures (B.loc_in (footprint m s) m))
+  [SMTPat (invariant m s)]
+
+/// Ghost accessors
+/// ---------------
+///
+/// We need to define those, so that we can state a framing lemma for them.
+/// Attempting a new convention to distinguish ghost accessors from stateful
+/// functions: a ``g_`` prefix.
+
+val g_aead_key: #i:index -> (s: state_s i) -> (h: HS.mem) -> Spec.AEAD.kv i.aead_alg
+val g_static_iv: #i:index -> (s: state_s i) -> (h: HS.mem) -> lbytes 12
+val g_counter: #i:index -> (s: state_s i) -> (h: HS.mem) -> Spec.QUIC.nat62
+val g_hash: #i:index -> (s: state_s i) -> (h: HS.mem) -> Spec.Hash.Definitions.bytes_hash i.hash_alg
+
+/// Preserving all the ghost accessors via a single framing lemma only works
+/// because we don't do stack allocation. See comments in
+/// EverCrypt.Hash.Incremental.
+val frame_invariant: #i:index -> l:B.loc -> s:state i -> h0:HS.mem -> h1:HS.mem -> Lemma
+  (requires (
+    invariant h0 s /\
+    B.loc_disjoint l (footprint h0 s) /\
+    B.modifies l h0 h1))
+  (ensures (
+    invariant h1 s /\
+    footprint h0 s == footprint h1 s /\
+    g_aead_key (B.deref h0 s) == g_aead_key (B.deref h1 s) /\
+    g_static_iv (B.deref h0 s) == g_static_iv (B.deref h1 s) /\
+    g_counter (B.deref h0 s) == g_counter (B.deref h1 s) /\
+    g_hash (B.deref h0 s) == g_hash (B.deref h1 s)
+    ))
+  // Assertion failure: unexpected pattern term
+  (*[ SMTPat (B.modifies l h0 h1); SMTPatOr [
+    [ SMTPat (invariant h1 s) ];
+    [ SMTPat (footprint h1 s) ];
+    [ SMTPat (g_aead_key (B.deref h1 s)) ];
+    [ SMTPat (g_static_iv (B.deref h1 s)) ];
+    [ SMTPat (g_counter (B.deref h1 s)) ]
+  ]]*)
+
+/// Actual stateful API
+/// -------------------
+///
+/// Note that we do not store the role at run-time, since the representation is
+/// the same regardless of the role. It's just the *interpretation* of the
+/// packet number that varies according to the role.
+
+val aead_alg_of_state (i: G.erased index) (s: state (G.reveal i)): Stack aead_alg
+  (requires (fun h0 -> invariant #(G.reveal i) h0 s))
+  (ensures (fun h0 a h1 ->
+    a == (G.reveal i).aead_alg /\
+    h0 == h1))
+
+val hash_alg_of_state (i: G.erased index) (s: state (G.reveal i)): Stack hash_alg
+  (requires (fun h0 -> invariant #(G.reveal i) h0 s))
+  (ensures (fun h0 a h1 ->
+    a == (G.reveal i).hash_alg /\
+    h0 == h1))
+
+// TODO: move to spec
+val label_key : Spec.QUIC.lbytes 3
+val label_iv : Spec.QUIC.lbytes 2
+val label_hp : Spec.QUIC.lbytes 2
+
+val encrypt: #i:G.erased index -> (
+  let i = G.reveal i in
+  s: state i ->
+  dst: B.buffer U8.t ->
+  h: header ->
+  plain: B.buffer U8.t ->
+  plain_len: U32.t {
+    3 <= U32.v plain_len /\
+    U32.v plain_len < Spec.QUIC.max_plain_length /\
+    B.length plain = U32.v plain_len
+  } ->
+  pn_len: u2 ->
+  Stack error_code
+    (requires fun h0 ->
+      // Memory & preservation
+      B.live h0 plain /\ B.live h0 dst /\
+      B.disjoint plain dst /\ // JP: probably needed, along with many others
+      invariant h0 s /\
+
+      i.role = Writer /\
+      // TODO: same length condition as in QuicCrypto.fsti
+
+      True)
+    (ensures fun h0 r h1 ->
+      // Memory & preservation
+      B.modifies (footprint h0 s) h0 h1 /\
+      invariant h1 s /\
+      footprint h1 s == footprint h0 s /\ (
+
+      // Functional correctness
+      let s0 = g_hash (B.deref h0 s) in
+      let k = Spec.QUIC.derive_secret i.hash_alg s0 label_key (Spec.AEAD.key_length a.ea) in
+      let iv = Spec.QUIC.derive_secret i.hash_alg s0 label_iv 12 in
+      let pne = Spec.QUIC.derive_secret i.hash_alg s0 label_hp (Spec.QUIC.ae_keysize a.ea) in
+      let plain: Spec.QUIC.pbytes = B.as_seq h0 plain in
+      let packet: Spec.QUIC.packet = B.as_seq h1 out in
+      let ctr = pnT s Writer h0 in
+      packet == Spec.QUIC.encrypt a.ea k iv pne (U8.v pn_len) ctr (spec_header h h0) plain)))
